wellorder instance

Ordered_Resolution_Prover/IsaFoR_IsaFoR_Term.thy
@@ -13,7 +13,147 @@ theory IsaFoR_IsaFoR_Term
     "../lib/Explorer" (* FIXME: remove explorer when done *)
     "$ISAFOR/Normalization_Equivalence/Encompassment" (* Version 7a339721b8c2 *)
     "./AFP_IsaFoR/Fun_More"
+    "$ISAFOR/Orderings/KBO" (*_Impl*)
 begin
+
+record 'f weights =
+  w :: "'f \<times> nat \<Rightarrow> nat"
+  w0 :: nat
+  pr_strict :: "'f \<times> nat \<Rightarrow> 'f \<times> nat \<Rightarrow> bool"
+  least :: "'f \<Rightarrow> bool"
+  scf :: "'f \<times> nat \<Rightarrow> nat \<Rightarrow> nat"
+
+class weighted =
+  fixes weights :: "'a weights"
+  assumes weights_adm:
+    "admissible_weight_fun_prc
+       (w weights) (w0 weights) (pr_strict weights) ((pr_strict weights)\<^sup>=\<^sup>=) (least weights) (scf weights)"
+  and pr_strict_total: "fi = gj \<or> pr_strict weights fi gj \<or> pr_strict weights gj fi"
+  and pr_strict_asymp: "asymp (pr_strict weights)"
+  and scf_ok: "i < n \<Longrightarrow> scf weights (f, n) i \<le> 1"
+
+instantiation unit :: weighted begin
+
+definition weights_unit :: "unit weights" where "weights_unit =
+  \<lparr>w = Suc o snd, w0 = 1, pr_strict = \<lambda>(_, n) (_, m). n > m, least = \<lambda>_. True, scf = \<lambda>_ _. 1\<rparr>"
+
+instance
+  by (intro_classes, unfold_locales)
+    (auto simp: weights_unit_def SN_iff_wf asymp.simps irreflp_def
+               intro!: wf_subset[OF wf_inv_image[OF wf], of _ snd])
+end
+
+global_interpretation KBO:
+  admissible_weight_fun_prc
+    "w (weights :: 'f :: weighted weights)" "w0 (weights :: 'f :: weighted weights)"
+    "pr_strict weights" "((pr_strict weights)\<^sup>=\<^sup>=)" "least weights" "scf weights"
+    defines weight = KBO.weight
+    and gtkbo = KBO.gtkbo
+    and kbo = KBO.kbo
+  by (simp add: weights_adm)
+
+lemma kbo_code[code]: "kbo s t =
+  (let wt = weight t; ws = weight s in
+  if vars_term_ms (KBO.SCF t) \<subseteq># vars_term_ms (KBO.SCF s) \<and> wt \<le> ws
+  then
+    (if wt < ws then (True, True)
+    else
+      (case s of
+        Var y \<Rightarrow> (False, case t of Var x \<Rightarrow> True | Fun g ts \<Rightarrow> ts = [] \<and> least weights g)
+      | Fun f ss \<Rightarrow>
+          (case t of
+            Var x \<Rightarrow> (True, True)
+          | Fun g ts \<Rightarrow>
+              if pr_strict weights (f, length ss) (g, length ts) then (True, True)
+              else if (f, length ss) = (g, length ts) then lex_ext_unbounded kbo ss ts
+              else (False, False))))
+  else (False, False))"
+  by (subst KBO.kbo.simps) (auto simp: Let_def split: term.splits)
+
+definition "less_kbo s t = fst (kbo t s)"
+
+lemma less_kbo_gtkbo: "ground s \<Longrightarrow> ground t \<Longrightarrow> less_kbo s t = gtkbo t s"
+  unfolding less_kbo_def using KBO.kbo_eq_gtkbo[OF refl pr_strict_total, of t s] by auto
+
+lemma less_kbo_gtotal: "ground s \<Longrightarrow> ground t \<Longrightarrow> s = t \<or> less_kbo s t \<or> less_kbo t s"
+  using less_kbo_gtkbo KBO.gtkbo_gtotal[OF refl pr_strict_total subset_UNIV _ subset_UNIV] by blast
+
+lemma less_kbo_subst:
+  fixes \<sigma> :: "('f :: weighted, 'v) subst"
+  shows "less_kbo s t \<Longrightarrow> less_kbo (s \<cdot> \<sigma>) (t \<cdot> \<sigma>)"
+  unfolding less_kbo_def by (rule KBO.S_subst)
+
+lemma wfP_less_kbo:
+  "wfP less_kbo"
+proof -
+  have "SN {(x, y). fst (kbo x y)}"
+    using pr_strict_asymp by (fastforce simp: asymp.simps irreflp_def intro!: KBO.SN_S_po scf_ok)
+  then show ?thesis
+    unfolding SN_iff_wf wfP_def by (rule wf_subset) (auto simp: less_kbo_def)
+qed
+
+instantiation "term" :: (weighted, type) linorder begin
+
+definition "leq_term = (SOME leq. {(s,t). less_kbo s t} \<subseteq> leq \<and> Well_order leq \<and> Field leq = UNIV)"
+
+lemma less_trm_extension: "{(s,t). less_kbo s t} \<subseteq> leq_term"
+  unfolding leq_term_def
+  by (rule someI2_ex[OF total_well_order_extension[OF wfP_less_kbo[unfolded wfP_def]]]) auto
+
+lemma less_trm_well_order: "well_order leq_term"
+  unfolding leq_term_def
+  by (rule someI2_ex[OF total_well_order_extension[OF wfP_less_kbo[unfolded wfP_def]]]) auto
+
+definition less_eq_term :: "('a :: weighted, 'b) term \<Rightarrow> _ \<Rightarrow> bool" where
+  "less_eq_term = in_rel leq_term"
+definition less_term :: "('a :: weighted, 'b) term \<Rightarrow> _ \<Rightarrow> bool" where
+  "less_term s t = strict (op \<le>) s t"
+
+lemma leq_term_minus_Id: "leq_term - Id = {(x,y). x < y}"
+  using less_trm_well_order
+  unfolding well_order_on_def linear_order_on_def partial_order_on_def antisym_def less_term_def less_eq_term_def
+  by auto
+
+instance
+proof (standard, goal_cases less_less_eq refl trans antisym total)
+  case (less_less_eq x y)
+  then show ?case unfolding less_term_def ..
+next
+case (refl x)
+  then show ?case using less_trm_well_order
+    unfolding well_order_on_def linear_order_on_def partial_order_on_def preorder_on_def refl_on_def
+      less_eq_term_def by auto
+next
+case (trans x y z)
+  then show ?case using less_trm_well_order
+    unfolding well_order_on_def linear_order_on_def partial_order_on_def preorder_on_def trans_def
+      less_eq_term_def by auto
+next
+  case (antisym x y)
+  then show ?case using less_trm_well_order
+    unfolding well_order_on_def linear_order_on_def partial_order_on_def antisym_def
+      less_eq_term_def by auto
+next
+  case (total x y)
+  then show ?case using less_trm_well_order
+    unfolding well_order_on_def linear_order_on_def partial_order_on_def preorder_on_def refl_on_def
+      Relation.total_on_def less_eq_term_def by (cases "x = y") auto
+qed
+
+end
+
+derive linorder prod
+derive linorder list
+
+instantiation "term" :: (weighted, type) wellorder begin
+instance
+  using less_trm_well_order[unfolded well_order_on_def wf_def leq_term_minus_Id, THEN conjunct2]
+  by intro_classes (atomize, auto)
+end
+
+lemma ground_less_less_kbo: "ground s \<Longrightarrow> ground t \<Longrightarrow> s < t \<Longrightarrow> less_kbo s t"
+  using less_kbo_gtotal[of s t] less_trm_extension
+  by (auto simp: less_term_def less_eq_term_def)
 
 abbreviation
   subst_apply_set :: "('f, 'v) terms \<Rightarrow> ('f, 'v, 'w) gsubst \<Rightarrow> ('f, 'w) terms" (infixl "\<cdot>\<^sub>s\<^sub>e\<^sub>t" 60)
@@ -21,10 +161,6 @@ abbreviation
     "T \<cdot>\<^sub>s\<^sub>e\<^sub>t \<sigma> \<equiv> (\<lambda>t. t \<cdot> \<sigma>) ` T"
 
 hide_const (open) mgu
-
-derive linorder prod
-derive linorder list
-derive linorder "term"
 
 abbreviation subst_apply_literal :: "('f, 'v) term literal \<Rightarrow> ('f, 'v, 'w) gsubst \<Rightarrow> ('f, 'w) term literal" (infixl "\<cdot>lit" 60) where
   "L \<cdot>lit \<sigma> \<equiv> map_literal (\<lambda>A. A \<cdot> \<sigma>) L"
@@ -607,16 +743,16 @@ qed
 
 definition "mgu_sets AAA = map_option subst_of (unify (Pairs AAA) [])"
 
-interpretation mgu "op \<cdot>" "Var :: _ \<Rightarrow> ('f :: linorder, nat) term" "op \<circ>\<^sub>s" "Fun undefined" renamings_apart mgu_sets
+interpretation mgu "op \<cdot>" "Var :: _ \<Rightarrow> ('f :: weighted, nat) term" "op \<circ>\<^sub>s" "Fun undefined" renamings_apart mgu_sets
 proof
-  fix AAA :: "('a :: linorder, nat) term set set" and \<sigma> :: "('a, nat) subst"
+  fix AAA :: "('a :: weighted, nat) term set set" and \<sigma> :: "('a, nat) subst"
   assume fin: "finite AAA" "\<forall>AA\<in>AAA. finite AA" and "mgu_sets AAA = Some \<sigma>"
   then have "is_imgu \<sigma> (set (Pairs AAA))"
     using unify_sound unfolding mgu_sets_def by blast
   then show "is_mgu \<sigma> AAA"
     unfolding is_imgu_def is_mgu_def unifiers_Pairs[OF fin] by auto
 next
-  fix AAA :: "('a :: linorder, nat) term set set" and \<sigma> :: "('a, nat) subst"
+  fix AAA :: "('a :: weighted, nat) term set set" and \<sigma> :: "('a, nat) subst"
   assume fin: "finite AAA" "\<forall>AA\<in>AAA. finite AA" and "is_unifiers \<sigma> AAA"
   then have "\<sigma> \<in> unifiers (set (Pairs AAA))"
     unfolding is_mgu_def unifiers_Pairs[OF fin] by auto
