Ordered_Resolution_Prover/Executable_FO_Ordered_Resolution_Prover.thy
@@ -10,14 +10,10 @@ TODO.
 \<close>
 
 theory Executable_FO_Ordered_Resolution_Prover
-  imports Deterministic_FO_Ordered_Resolution_Prover IsaFoR_Term
+  imports Deterministic_FO_Ordered_Resolution_Prover IsaFoR_IsaFoR_Term
 begin
-
-instantiation "term" :: (wellorder, wellorder) wellorder begin
-instance sorry
-end
-
-interpretation deterministic_FO_resolution_prover S
+thm deterministic_FO_resolution_prover
+global_interpretation deterministic_FO_resolution_prover "\<lambda>_. {#}"
   "op \<cdot>" "Var :: _ \<Rightarrow> ('f :: wellorder, nat) term" "op \<circ>\<^sub>s" renamings_apart "Fun undefined" mgu_sets
   apply (intro_locales)
 
